Kuiper.Common: divmod

src/lib/kuiper/Kuiper.Common.fsti
@@ -14,3 +14,16 @@ type szlt (n:nat) = i:FStar.SizeT.t{FStar.SizeT.v i < n}
 (* really just ez = easy *)
 let ez : #a:Type -> (#[Tactics.V2.easy_fill ()] _ : a) -> a = Tactics.V2.easy
 
+let divmod (j:pos) (i : nat) : (nat & natlt j) =
+  (i / j, i % j)
+
+let undivmod (j:pos) (xy : nat & natlt j) : nat =
+  j * xy._1 + xy._2
+
+let divmod_inv_1 (j:pos) (i:nat)
+  : Lemma (undivmod j (divmod j i) == i)
+  = ()
+
+let divmod_inv_2 (j:pos) (xy : nat & natlt j)
+  : Lemma (divmod j (undivmod j xy) == xy)
+  = ()
